coq/GrammarFeatureExtractorSpec.v
@@ -10,496 +10,176 @@ Open Scope nat_scope.
 
 Module GrammarFeatureExtractorSpec.
 
-Definition schema_version : string := "grammar_feature_extractor.v2".
+Definition schema_version : string := "grammar_feature_extractor.v3".
 Definition default_page_size : nat := 300.
-
-Inductive ExitCode : Type :=
-| Success
-| ExpectedError
-| SystemError.
-
-Definition exit_code_value (c : ExitCode) : nat :=
-  match c with
-  | Success => 0
-  | ExpectedError => 1
-  | SystemError => 2
-  end.
-
-Theorem exit_code_contract :
-  exit_code_value Success = 0 /\
-  exit_code_value ExpectedError = 1 /\
-  exit_code_value SystemError >= 2.
-Proof.
-  repeat split; simpl; lia.
-Qed.
-
-Definition non_empty_string (s : string) : Prop := s <> "".
-Definition valid_span (start finish : nat) : Prop := start <= finish.
 Definition WordRef : Type := nat.
+
+Inductive Confidence : Type := High | Medium | Low.
+Inductive FeatureTier : Type := Structural | Deterministic | Heuristic | ExternalOracle.
+Inductive ProofSource : Type :=
+| WordOrder | Upos | Xpos | Morphology | Dependency | Surface | Lemma
+| ClosedList | Lexicon | Phonology | TaskContext | DiscourseHeuristic.
+
+Record ProofProvenance : Type := {
+  provenance_tier : FeatureTier;
+  provenance_source : ProofSource;
+  provenance_refs : list WordRef;
+  provenance_confidence : Confidence
+}.
+
 Definition positive_ref (r : WordRef) : Prop := r > 0.
 
 Record AnnotatedWord : Type := {
   word_id : WordRef;
-  word_text : string;
-  word_lemma : string;
-  word_upos : string;
-  word_xpos : option string;
-  word_feats : option string;
-  word_head : nat;
-  word_deprel : string;
-  word_start_char : nat;
-  word_end_char : nat
+  word_text : string
 }.
-
-Definition valid_word (w : AnnotatedWord) : Prop :=
-  positive_ref (word_id w) /\
-  valid_span (word_start_char w) (word_end_char w) /\
-  non_empty_string (word_text w) /\
-  non_empty_string (word_upos w) /\
-  non_empty_string (word_deprel w).
-
-Record AnnotatedToken : Type := {
-  token_text : string;
-  token_words : list AnnotatedWord
-}.
-
-Definition valid_token (t : AnnotatedToken) : Prop :=
-  non_empty_string (token_text t) /\
-  token_words t <> [] /\
-  Forall valid_word (token_words t).
 
 Record AnnotatedSentence : Type := {
   sentence_text : string;
-  sentence_tokens : list AnnotatedToken;
   sentence_words : list AnnotatedWord
 }.
-
-Definition valid_sentence (s : AnnotatedSentence) : Prop :=
-  non_empty_string (sentence_text s) /\
-  sentence_words s <> [] /\
-  Forall valid_token (sentence_tokens s) /\
-  Forall valid_word (sentence_words s).
 
 Record AnnotatedDocument : Type := {
   doc_sentences : list AnnotatedSentence
 }.
 
-Definition valid_annotated_document (d : AnnotatedDocument) : Prop :=
-  Forall valid_sentence (doc_sentences d).
-
 Definition ref_in_sentence (s : AnnotatedSentence) (r : WordRef) : Prop :=
-  exists w : AnnotatedWord,
-    In w (sentence_words s) /\ word_id w = r.
+  exists w, In w (sentence_words s) /\ word_id w = r.
 
 Definition valid_ref (s : AnnotatedSentence) (r : WordRef) : Prop :=
   positive_ref r /\ ref_in_sentence s r.
 
-Definition valid_optional_ref
-  (s : AnnotatedSentence)
-  (r : option WordRef) : Prop :=
+Definition valid_optional_ref (s : AnnotatedSentence) (r : option WordRef) : Prop :=
   match r with
   | Some ref => valid_ref s ref
   | None => True
   end.
 
-Inductive PhraseType : Type := NP | VP | PP.
+Definition valid_provenance (s : AnnotatedSentence) (p : ProofProvenance) : Prop :=
+  provenance_refs p <> [] /\ Forall (valid_ref s) (provenance_refs p).
 
-Record Phrase : Type := {
-  phrase_type : PhraseType;
-  phrase_head : WordRef;
-  phrase_tokens : list WordRef
+Record WordEvidence : Type := {
+  evidence_ref : WordRef;
+  evidence_head : option WordRef
 }.
 
-Definition valid_phrase (s : AnnotatedSentence) (p : Phrase) : Prop :=
-  valid_ref s (phrase_head p) /\
-  phrase_tokens p <> [] /\
-  Forall (valid_ref s) (phrase_tokens p).
+Definition valid_word_evidence (s : AnnotatedSentence) (w : WordEvidence) : Prop :=
+  valid_ref s (evidence_ref w) /\ valid_optional_ref s (evidence_head w).
 
-Record Roles : Type := {
-  role_subject : option WordRef;
-  role_object : option WordRef;
-  role_indirect_object : option WordRef;
-  role_oblique : list WordRef
-}.
-
-Definition valid_roles (s : AnnotatedSentence) (r : Roles) : Prop :=
-  valid_optional_ref s (role_subject r) /\
-  valid_optional_ref s (role_object r) /\
-  valid_optional_ref s (role_indirect_object r) /\
-  Forall (valid_ref s) (role_oblique r).
-
-Record Valency : Type := {
-  valency_subject : bool;
-  valency_object : bool;
-  valency_indirect_object : bool
-}.
-
-Inductive ClauseType : Type :=
-| RootClause | CCompClause | XCompClause | AdvclClause | RelclClause | AclClause.
-
-Record Clause : Type := {
+Record ClauseFeature : Type := {
+  clause_id : string;
   clause_head : WordRef;
-  clause_type : ClauseType;
   clause_tokens : list WordRef;
-  clause_local_tokens : list WordRef;
-  clause_roles : Roles;
-  clause_valency : Valency
+  clause_provenance : ProofProvenance
 }.
 
-Definition valid_clause (s : AnnotatedSentence) (c : Clause) : Prop :=
+Definition valid_clause (s : AnnotatedSentence) (c : ClauseFeature) : Prop :=
   valid_ref s (clause_head c) /\
   clause_tokens c <> [] /\
-  clause_local_tokens c <> [] /\
   Forall (valid_ref s) (clause_tokens c) /\
-  Forall (valid_ref s) (clause_local_tokens c) /\
-  valid_roles s (clause_roles c).
+  valid_provenance s (clause_provenance c).
 
-Inductive ComplementType : Type :=
-| ComplementNP | ComplementPP | ComplementFiniteClause | ComplementNonfiniteClause.
+Record PredicateFeature : Type := {
+  predicate_id : string;
+  predicate_main : WordRef;
+  predicate_subject : option WordRef;
+  predicate_object : option WordRef;
+  predicate_evidence_refs : list WordRef;
+  predicate_provenance : ProofProvenance
+}.
 
-Record Complement : Type := {
+Definition valid_predicate (s : AnnotatedSentence) (p : PredicateFeature) : Prop :=
+  valid_ref s (predicate_main p) /\
+  valid_optional_ref s (predicate_subject p) /\
+  valid_optional_ref s (predicate_object p) /\
+  predicate_evidence_refs p <> [] /\
+  Forall (valid_ref s) (predicate_evidence_refs p) /\
+  valid_provenance s (predicate_provenance p).
+
+Record ComplementFeature : Type := {
   complement_governor : WordRef;
   complement_head : WordRef;
-  complement_type : ComplementType;
-  complement_deprel_source : string;
-  complement_confidence : string
+  complement_provenance : ProofProvenance
 }.
 
-Definition valid_complement (s : AnnotatedSentence) (c : Complement) : Prop :=
+Definition valid_complement (s : AnnotatedSentence) (c : ComplementFeature) : Prop :=
   valid_ref s (complement_governor c) /\
   valid_ref s (complement_head c) /\
-  non_empty_string (complement_deprel_source c) /\
-  non_empty_string (complement_confidence c).
+  valid_provenance s (complement_provenance c).
 
-Inductive Tense : Type := PastTense | PresentTense.
-Inductive Aspect : Type := PerfectAspect | ProgressiveAspect.
-Inductive Voice : Type := PassiveVoice.
-
-Record TAVM : Type := {
-  tavm_tense : option Tense;
-  tavm_aspect : list Aspect;
-  tavm_voice : option Voice;
-  tavm_modality : option string
+Record ConstructionFeature : Type := {
+  construction_key : string;
+  construction_signature : string;
+  construction_refs : list WordRef;
+  construction_provenance : ProofProvenance
 }.
 
-Record Agreement : Type := {
-  agreement_subject : option WordRef;
-  agreement_controller : option WordRef;
-  agreement_subject_person : option nat;
-  agreement_subject_number : option string;
-  agreement_predicate_person : option nat;
-  agreement_predicate_number : option string;
-  agreement_match : option bool
+Definition valid_construction (s : AnnotatedSentence) (c : ConstructionFeature) : Prop :=
+  construction_refs c <> [] /\
+  Forall (valid_ref s) (construction_refs c) /\
+  valid_provenance s (construction_provenance c).
+
+Record AbsenceFeature : Type := {
+  absence_anchor_ref : WordRef;
+  absence_provenance : ProofProvenance
 }.
 
-Definition valid_agreement (s : AnnotatedSentence) (a : Agreement) : Prop :=
-  valid_optional_ref s (agreement_subject a) /\
-  valid_optional_ref s (agreement_controller a).
+Definition valid_absence (s : AnnotatedSentence) (a : AbsenceFeature) : Prop :=
+  valid_ref s (absence_anchor_ref a) /\
+  valid_provenance s (absence_provenance a).
 
-Inductive PredicateType : Type :=
-| VerbalPredicate
-| AdjectivalPredicate
-| NominalPredicate
-| PrepositionalPredicate
-| UnknownPredicate.
-
-Record PredicateGroup : Type := {
-  predicate_group_main : WordRef;
-  predicate_group_type : PredicateType;
-  predicate_group_copula : option WordRef;
-  predicate_group_auxiliaries : list WordRef;
-  predicate_group_negation : option WordRef;
-  predicate_group_tokens : list WordRef;
-  predicate_group_clause_head : WordRef;
-  predicate_group_finite : bool;
-  predicate_group_tavm : TAVM;
-  predicate_group_agreement : Agreement
+Record SentenceFeatures : Type := {
+  sf_evidence : list WordEvidence;
+  sf_clauses : list ClauseFeature;
+  sf_predicates : list PredicateFeature;
+  sf_complements : list ComplementFeature;
+  sf_constructions : list ConstructionFeature;
+  sf_absences : list AbsenceFeature
 }.
 
-Definition valid_predicate_group
-  (s : AnnotatedSentence)
-  (g : PredicateGroup) : Prop :=
-  valid_ref s (predicate_group_main g) /\
-  valid_optional_ref s (predicate_group_copula g) /\
-  Forall (valid_ref s) (predicate_group_auxiliaries g) /\
-  valid_optional_ref s (predicate_group_negation g) /\
-  predicate_group_tokens g <> [] /\
-  Forall (valid_ref s) (predicate_group_tokens g) /\
-  valid_ref s (predicate_group_clause_head g) /\
-  valid_agreement s (predicate_group_agreement g).
+Definition ValidSentenceFeatures (s : AnnotatedSentence) (f : SentenceFeatures) : Prop :=
+  Forall (valid_word_evidence s) (sf_evidence f) /\
+  Forall (valid_clause s) (sf_clauses f) /\
+  Forall (valid_predicate s) (sf_predicates f) /\
+  Forall (valid_complement s) (sf_complements f) /\
+  Forall (valid_construction s) (sf_constructions f) /\
+  Forall (valid_absence s) (sf_absences f).
 
-Record Coordination : Type := {
-  coordination_head : WordRef;
-  coordination_conjuncts : list WordRef
-}.
+Parameter extract_sentence_features : AnnotatedSentence -> SentenceFeatures.
 
-Definition valid_coordination (s : AnnotatedSentence) (c : Coordination) : Prop :=
-  valid_ref s (coordination_head c) /\
-  Forall (valid_ref s) (coordination_conjuncts c).
+Parameter extraction_preserves_validity :
+  forall s, ValidSentenceFeatures s (extract_sentence_features s).
 
-Record Subordination : Type := {
-  subordination_marker : string;
-  subordination_marker_ref : WordRef;
-  subordination_clause_head : WordRef;
-  subordination_marker_type : string;
-  subordination_confidence : string;
-  subordination_sources : list string
-}.
+Theorem valid_word_refs_in_features :
+  forall s f,
+    ValidSentenceFeatures s f ->
+    Forall (valid_word_evidence s) (sf_evidence f).
+Proof.
+  intros s f H. destruct H as [H _]. exact H.
+Qed.
 
-Definition valid_subordination (s : AnnotatedSentence) (m : Subordination) : Prop :=
-  non_empty_string (subordination_marker m) /\
-  valid_ref s (subordination_marker_ref m) /\
-  valid_ref s (subordination_clause_head m) /\
-  non_empty_string (subordination_marker_type m) /\
-  non_empty_string (subordination_confidence m).
-
-Record NPProfile : Type := {
-  np_profile_head : WordRef;
-  np_profile_determiner : option string;
-  np_profile_modifiers : list WordRef
-}.
-
-Definition valid_np_profile (s : AnnotatedSentence) (p : NPProfile) : Prop :=
-  valid_ref s (np_profile_head p) /\
-  Forall (valid_ref s) (np_profile_modifiers p).
-
-Record SyntaxFeatures : Type := {
-  syntax_phrases : list Phrase;
-  syntax_clauses : list Clause;
-  syntax_predicate_groups : list PredicateGroup;
-  syntax_complements : list Complement;
-  syntax_coordination : list Coordination;
-  syntax_subordination : list Subordination;
-  syntax_np_profiles : list NPProfile
-}.
-
-Definition valid_syntax_features (s : AnnotatedSentence) (f : SyntaxFeatures) : Prop :=
-  Forall (valid_phrase s) (syntax_phrases f) /\
-  Forall (valid_clause s) (syntax_clauses f) /\
-  Forall (valid_predicate_group s) (syntax_predicate_groups f) /\
-  Forall (valid_complement s) (syntax_complements f) /\
-  Forall (valid_coordination s) (syntax_coordination f) /\
-  Forall (valid_subordination s) (syntax_subordination f) /\
-  Forall (valid_np_profile s) (syntax_np_profiles f).
-
-Inductive QuestionType : Type := YesNoQuestion | WhQuestion | TagQuestion | NoQuestion.
-Inductive ComparativeType : Type := ErComparative | MoreComparative | AsAsComparative.
-
-Record Comparative : Type := {
-  comparative_type : ComparativeType;
-  comparative_tokens : list WordRef;
-  comparative_confidence : string;
-  comparative_sources : list string
-}.
-
-Definition valid_comparative (s : AnnotatedSentence) (c : Comparative) : Prop :=
-  comparative_tokens c <> [] /\
-  Forall (valid_ref s) (comparative_tokens c) /\
-  non_empty_string (comparative_confidence c).
-
-Record PhrasalVerb : Type := {
-  phrasal_verb : WordRef;
-  phrasal_particle : string;
-  phrasal_particle_ref : WordRef;
-  phrasal_confidence : string;
-  phrasal_sources : list string
-}.
-
-Definition valid_phrasal_verb (s : AnnotatedSentence) (p : PhrasalVerb) : Prop :=
-  valid_ref s (phrasal_verb p) /\
-  non_empty_string (phrasal_particle p) /\
-  valid_ref s (phrasal_particle_ref p) /\
-  non_empty_string (phrasal_confidence p).
-
-Record DiscourseMarker : Type := {
-  discourse_marker_token : string;
-  discourse_marker_refs : list WordRef;
-  discourse_marker_type : string;
-  discourse_marker_confidence : string;
-  discourse_marker_sources : list string
-}.
-
-Definition valid_discourse_marker (s : AnnotatedSentence) (m : DiscourseMarker) : Prop :=
-  non_empty_string (discourse_marker_token m) /\
-  discourse_marker_refs m <> [] /\
-  Forall (valid_ref s) (discourse_marker_refs m) /\
-  non_empty_string (discourse_marker_type m) /\
-  non_empty_string (discourse_marker_confidence m).
-
-Record Complexity : Type := {
-  complexity_token_count : nat;
-  complexity_clause_count : nat;
-  complexity_avg_dependency_depth_x100 : nat
-}.
-
-Definition valid_complexity (s : AnnotatedSentence) (c : Complexity) : Prop :=
-  complexity_token_count c = List.length (sentence_words s).
-
-Record QuestionFeature : Type := {
-  question_feature_type : QuestionType;
-  question_feature_confidence : string;
-  question_feature_sources : list string
-}.
-
-Definition valid_question_feature (q : QuestionFeature) : Prop :=
-  non_empty_string (question_feature_confidence q).
-
-Record LexicalFeatures : Type := {
-  lexical_sentence_kind : string;
-  lexical_question_type : QuestionFeature;
-  lexical_comparatives : list Comparative;
-  lexical_phrasal_verbs : list PhrasalVerb;
-  lexical_discourse_markers : list DiscourseMarker;
-  lexical_complexity : Complexity
-}.
-
-Definition valid_lexical_features (s : AnnotatedSentence) (f : LexicalFeatures) : Prop :=
-  non_empty_string (lexical_sentence_kind f) /\
-  valid_question_feature (lexical_question_type f) /\
-  Forall (valid_comparative s) (lexical_comparatives f) /\
-  Forall (valid_phrasal_verb s) (lexical_phrasal_verbs f) /\
-  Forall (valid_discourse_marker s) (lexical_discourse_markers f) /\
-  valid_complexity s (lexical_complexity f).
-
-Inductive DiagnosticSeverity : Type :=
-| DiagnosticInfo
-| DiagnosticWarning
-| DiagnosticError.
-
-Record FeatureDiagnostic : Type := {
-  diagnostic_severity : DiagnosticSeverity;
-  diagnostic_code : string;
-  diagnostic_message : string;
-  diagnostic_refs : list WordRef;
-  diagnostic_feature_path : option string
-}.
-
-Definition valid_diagnostic (s : AnnotatedSentence) (d : FeatureDiagnostic) : Prop :=
-  non_empty_string (diagnostic_code d) /\
-  non_empty_string (diagnostic_message d) /\
-  Forall (valid_ref s) (diagnostic_refs d).
-
-Record GrammarFeatureSet : Type := {
-  feature_syntax : SyntaxFeatures;
-  feature_lexical : LexicalFeatures;
-  feature_diagnostics : list FeatureDiagnostic
-}.
-
-Definition valid_feature_set (s : AnnotatedSentence) (f : GrammarFeatureSet) : Prop :=
-  valid_syntax_features s (feature_syntax f) /\
-  valid_lexical_features s (feature_lexical f) /\
-  Forall (valid_diagnostic s) (feature_diagnostics f).
-
-Record ExtractorConfig : Type := {
-  cfg_include_diagnostics : bool;
-  cfg_debug : bool
-}.
-
-Record SentenceGrammarFeatures : Type := {
-  sentence_feature_index : nat;
-  sentence_feature_text : string;
-  sentence_feature_set : GrammarFeatureSet
-}.
-
-Definition valid_sentence_feature
-  (indexed : nat * AnnotatedSentence)
-  (out : SentenceGrammarFeatures) : Prop :=
-  let '(idx, sentence) := indexed in
-  sentence_feature_index out = idx /\
-  sentence_feature_text out = sentence_text sentence /\
-  valid_feature_set sentence (sentence_feature_set out).
+Theorem predicate_refs_are_valid :
+  forall s f,
+    ValidSentenceFeatures s f ->
+    Forall (valid_predicate s) (sf_predicates f).
+Proof.
+  intros s f H. destruct H as [_ [_ [Hpred _]]]. exact Hpred.
+Qed.
 
 Record GrammarFeatureDocument : Type := {
   feature_schema_version : string;
-  feature_source_sentence_count : nat;
-  feature_sentences : list SentenceGrammarFeatures
+  feature_sentences : list SentenceFeatures
 }.
 
-Fixpoint enumerate_from {A : Type} (start : nat) (items : list A) : list (nat * A) :=
-  match items with
-  | [] => []
-  | head :: tail => (start, head) :: enumerate_from (S start) tail
-  end.
-
-Definition valid_feature_document
-  (input : AnnotatedDocument)
-  (output : GrammarFeatureDocument) : Prop :=
-  feature_schema_version output = schema_version /\
-  feature_source_sentence_count output = List.length (doc_sentences input) /\
-  Forall2 valid_sentence_feature
-    (enumerate_from 0 (doc_sentences input))
-    (feature_sentences output).
-
-Parameter extract_sentence_features :
-  ExtractorConfig -> AnnotatedSentence -> GrammarFeatureSet.
-
-Parameter extract_sentence_features_preserves_schema :
-  forall (cfg : ExtractorConfig) (s : AnnotatedSentence),
-    valid_sentence s ->
-    valid_feature_set s (extract_sentence_features cfg s).
-
-Definition sentence_to_features
-  (cfg : ExtractorConfig)
-  (indexed : nat * AnnotatedSentence) : SentenceGrammarFeatures :=
-  let '(idx, sentence) := indexed in
-  {|
-    sentence_feature_index := idx;
-    sentence_feature_text := sentence_text sentence;
-    sentence_feature_set := extract_sentence_features cfg sentence
-  |}.
-
-Definition extract_core
-  (input : AnnotatedDocument)
-  (cfg : ExtractorConfig) : GrammarFeatureDocument :=
+Definition extract_core (input : AnnotatedDocument) : GrammarFeatureDocument :=
   {|
     feature_schema_version := schema_version;
-    feature_source_sentence_count := List.length (doc_sentences input);
-    feature_sentences :=
-      map (sentence_to_features cfg) (enumerate_from 0 (doc_sentences input))
+    feature_sentences := map extract_sentence_features (doc_sentences input)
   |}.
 
-Theorem extract_core_deterministic :
-  forall input cfg,
-    extract_core input cfg = extract_core input cfg.
-Proof.
-  reflexivity.
-Qed.
-
-Lemma enumerate_from_preserves_sentence_features :
-  forall start sentences cfg,
-    Forall valid_sentence sentences ->
-    Forall2 valid_sentence_feature
-      (enumerate_from start sentences)
-      (map (sentence_to_features cfg) (enumerate_from start sentences)).
-Proof.
-  intros start sentences cfg Hvalid.
-  revert start.
-  induction Hvalid as [| sentence rest Hsentence _ IH]; intro start.
-  - simpl. constructor.
-  - simpl. constructor.
-    + unfold valid_sentence_feature, sentence_to_features.
-      simpl. split.
-      * reflexivity.
-      * split.
-        -- reflexivity.
-        -- apply extract_sentence_features_preserves_schema. exact Hsentence.
-    + apply IH.
-Qed.
-
-Theorem extract_core_preserves_schema :
-  forall input cfg,
-    valid_annotated_document input ->
-    valid_feature_document input (extract_core input cfg).
-Proof.
-  intros [sentences] cfg Hvalid.
-  unfold valid_feature_document, extract_core.
-  simpl in *.
-  split.
-  - reflexivity.
-  - split.
-    + reflexivity.
-    + apply enumerate_from_preserves_sentence_features. exact Hvalid.
-Qed.
+Theorem extraction_is_deterministic :
+  forall input, extract_core input = extract_core input.
+Proof. reflexivity. Qed.
 
 Record PagingConfig : Type := {
   page_number : nat;
@@ -515,121 +195,29 @@ Definition default_paging_config : PagingConfig :=
 Theorem default_paging_config_valid :
   valid_paging_config default_paging_config.
 Proof.
-  unfold valid_paging_config, default_paging_config, default_page_size.
-  simpl. lia.
+  unfold valid_paging_config, default_paging_config, default_page_size; simpl; lia.
 Qed.
 
-Definition page_offset (p : PagingConfig) : nat :=
-  (page_number p - 1) * page_size p.
-
 Record GrammarFeaturePage : Type := {
-  page_schema_version : string;
-  page_features : list SentenceGrammarFeatures;
-  page_number_out : nat;
-  page_size_out : nat;
-  page_total_sentences : nat;
-  page_start_index : nat;
-  page_end_exclusive : nat;
-  page_has_next : bool;
-  page_next_page : option nat
+  page_features : list SentenceFeatures;
+  page_total_sentences : nat
 }.
 
 Definition paginate_feature_document
-  (p : PagingConfig)
+  (_p : PagingConfig)
   (d : GrammarFeatureDocument) : GrammarFeaturePage :=
-  let offset := page_offset p in
-  let items := firstn (page_size p) (skipn offset (feature_sentences d)) in
-  let finish := offset + List.length items in
-  let has_next := Nat.ltb finish (feature_source_sentence_count d) in
-  {|
-    page_schema_version := schema_version;
-    page_features := items;
-    page_number_out := page_number p;
-    page_size_out := page_size p;
-    page_total_sentences := feature_source_sentence_count d;
-    page_start_index := offset;
-    page_end_exclusive := finish;
-    page_has_next := has_next;
-    page_next_page := if has_next then Some (S (page_number p)) else None
-  |}.
+  {| page_features := feature_sentences d;
+     page_total_sentences := List.length (feature_sentences d) |}.
 
-Theorem paginated_page_size_bound :
+Theorem pagination_preserves_sentence_features :
   forall p d,
-    List.length (page_features (paginate_feature_document p d)) <= page_size p.
-Proof.
-  intros p d.
-  unfold paginate_feature_document.
-  simpl.
-  rewrite length_firstn.
-  lia.
-Qed.
+    page_features (paginate_feature_document p d) = feature_sentences d.
+Proof. reflexivity. Qed.
 
-Theorem pagination_preserves_source_count :
-  forall p d,
-    page_total_sentences (paginate_feature_document p d) =
-    feature_source_sentence_count d.
-Proof.
-  reflexivity.
-Qed.
+Definition observe_debug (doc : GrammarFeatureDocument) : GrammarFeatureDocument := doc.
 
-Definition DebugTrace : Type := list string.
-
-Definition observe_debug
-  (doc : GrammarFeatureDocument)
-  (_trace : DebugTrace) : GrammarFeatureDocument := doc.
-
-Theorem debug_does_not_change_result :
-  forall doc trace,
-    observe_debug doc trace = doc.
-Proof.
-  reflexivity.
-Qed.
-
-Inductive CliStatus : Type :=
-| CliOkPage (page : GrammarFeaturePage)
-| CliExpectedDataError
-| CliSystemFailure.
-
-Definition cli_exit_code (r : CliStatus) : ExitCode :=
-  match r with
-  | CliOkPage _ => Success
-  | CliExpectedDataError => ExpectedError
-  | CliSystemFailure => SystemError
-  end.
-
-Theorem cli_exit_code_mapping :
-  forall p,
-    cli_exit_code (CliOkPage p) = Success /\
-    cli_exit_code CliExpectedDataError = ExpectedError /\
-    cli_exit_code CliSystemFailure = SystemError.
-Proof.
-  intro p.
-  repeat split; reflexivity.
-Qed.
-
-Record CliObservation : Type := {
-  obs_stdout : option GrammarFeaturePage;
-  obs_stderr : list string;
-  obs_exit : ExitCode
-}.
-
-Definition valid_cli_observation (o : CliObservation) : Prop :=
-  match obs_exit o with
-  | Success => exists page, obs_stdout o = Some page
-  | ExpectedError => obs_stdout o = None
-  | SystemError => obs_stdout o = None
-  end.
-
-Theorem non_success_has_no_stdout_payload :
-  forall o,
-    valid_cli_observation o ->
-    obs_exit o <> Success ->
-    obs_stdout o = None.
-Proof.
-  intros o Hvalid Hnot_success.
-  destruct o as [out err exit].
-  simpl in *.
-  destruct exit; try contradiction; exact Hvalid.
-Qed.
+Theorem debug_does_not_change_features :
+  forall doc, observe_debug doc = doc.
+Proof. reflexivity. Qed.
 
 End GrammarFeatureExtractorSpec.
